Source/Core/Parser.cs
@@ -35,7 +35,7 @@ public class Parser {
 	public const int _decimal = 5;
 	public const int _dec_float = 6;
 	public const int _float = 7;
-	public const int maxT = 109;
+	public const int maxT = 110;
 
 	const bool _T = true;
 	const bool _x = false;
@@ -334,7 +334,7 @@ private class BvBounds : Expr {
 				axioms.Add(ax); 
 			}
 			Expect(26);
-		} else SynErr(110);
+		} else SynErr(111);
 		bool makeClone = false;
 		foreach(TypedIdent/*!*/ x in xs){
 		 Contract.Assert(x != null);
@@ -407,7 +407,7 @@ private class BvBounds : Expr {
 			Get();
 			Type(out retTy);
 			retTyd = new TypedIdent(retTy.tok, TypedIdent.NoName, retTy); 
-		} else SynErr(111);
+		} else SynErr(112);
 		if (la.kind == 25) {
 			Get();
 			Expression(out tmp);
@@ -432,7 +432,7 @@ private class BvBounds : Expr {
 			Expect(26);
 		} else if (la.kind == 9) {
 			Get();
-		} else SynErr(112);
+		} else SynErr(113);
 		if (retTyd == null) {
 		 // construct a dummy type for the case of syntax error
 		 retTyd = new TypedIdent(t, TypedIdent.NoName, new BasicType(t, SimpleType.Int));
@@ -566,7 +566,7 @@ private class BvBounds : Expr {
 			impl = new Implementation(x, x.val, typeParams.ConvertAll(tp => new TypeVariable(tp.tok, tp.Name)),
 			                         Formal.StripWhereClauses(ins), Formal.StripWhereClauses(outs), locals, stmtList, kv == null ? null : (QKeyValue)kv.Clone(), this.errors);
 			
-		} else SynErr(113);
+		} else SynErr(114);
 		proc = new Procedure(x, x.val, typeParams, ins, outs, pre, mods, post, kv); 
 	}
 
@@ -677,7 +677,7 @@ private class BvBounds : Expr {
 			ty = new UnresolvedTypeIdentifier (tok, tok.val, args); 
 		} else if (la.kind == 18 || la.kind == 20) {
 			MapType(out ty);
-		} else SynErr(114);
+		} else SynErr(115);
 	}
 
 	void AttributesIdsTypeWhere(bool allowAttributes, bool allowWhereClauses, string context, System.Action<TypedIdent, QKeyValue> action ) {
@@ -741,7 +741,7 @@ private class BvBounds : Expr {
 			Get();
 			Type(out ty);
 			Expect(11);
-		} else SynErr(115);
+		} else SynErr(116);
 	}
 
 	void Ident(out IToken/*!*/ x) {
@@ -771,7 +771,7 @@ private class BvBounds : Expr {
 		} else if (la.kind == 18 || la.kind == 20) {
 			MapType(out ty);
 			ts.Add(ty); 
-		} else SynErr(116);
+		} else SynErr(117);
 	}
 
 	void MapType(out Bpl.Type/*!*/ ty) {
@@ -956,7 +956,7 @@ out List<Variable>/*!*/ ins, out List<Variable>/*!*/ outs, out QKeyValue kv) {
 			SpecPrePost(true, pre, post);
 		} else if (la.kind == 38 || la.kind == 39) {
 			SpecPrePost(false, pre, post);
-		} else SynErr(117);
+		} else SynErr(118);
 	}
 
 	void ImplBody(out List<Variable>/*!*/ locals, out StmtList/*!*/ stmtList) {
@@ -988,7 +988,7 @@ out List<Variable>/*!*/ ins, out List<Variable>/*!*/ outs, out QKeyValue kv) {
 			Proposition(out e);
 			Expect(9);
 			post.Add(new Ensures(tok, free, e, null, kv)); 
-		} else SynErr(118);
+		} else SynErr(119);
 	}
 
 	void StmtList(out StmtList/*!*/ stmtList) {
@@ -1126,7 +1126,7 @@ out List<Variable>/*!*/ ins, out List<Variable>/*!*/ outs, out QKeyValue kv) {
 			c = new YieldCmd(x); 
 			break;
 		}
-		default: SynErr(119); break;
+		default: SynErr(120); break;
 		}
 	}
 
@@ -1143,7 +1143,7 @@ out List<Variable>/*!*/ ins, out List<Variable>/*!*/ outs, out QKeyValue kv) {
 		} else if (la.kind == 47) {
 			BreakCmd(out bcmd);
 			ec = bcmd; 
-		} else SynErr(120);
+		} else SynErr(121);
 	}
 
 	void TransferCmd(out TransferCmd/*!*/ tc) {
@@ -1163,7 +1163,7 @@ out List<Variable>/*!*/ ins, out List<Variable>/*!*/ outs, out QKeyValue kv) {
 		} else if (la.kind == 41) {
 			Get();
 			tc = new ReturnCmd(t); 
-		} else SynErr(121);
+		} else SynErr(122);
 		Expect(9);
 	}
 
@@ -1188,7 +1188,7 @@ out List<Variable>/*!*/ ins, out List<Variable>/*!*/ outs, out QKeyValue kv) {
 				Get();
 				StmtList(out els);
 				elseOption = els; 
-			} else SynErr(122);
+			} else SynErr(123);
 		}
 		ifcmd = new IfCmd(x, guard, thn, elseIfOption, elseOption); 
 	}
@@ -1252,7 +1252,7 @@ out List<Variable>/*!*/ ins, out List<Variable>/*!*/ outs, out QKeyValue kv) {
 		} else if (StartOf(9)) {
 			Expression(out ee);
 			e = ee; 
-		} else SynErr(123);
+		} else SynErr(124);
 		Expect(11);
 	}
 
@@ -1314,7 +1314,7 @@ out List<Variable>/*!*/ ins, out List<Variable>/*!*/ outs, out QKeyValue kv) {
 			}
 			Expect(9);
 			c = new AssignCmd(x, lhss, rhss, kv); 
-		} else SynErr(124);
+		} else SynErr(125);
 	}
 
 	void CallCmd(out Cmd c) {
@@ -1435,7 +1435,7 @@ out List<Variable>/*!*/ ins, out List<Variable>/*!*/ outs, out QKeyValue kv) {
 			}
 			Expect(11);
 			c = new CallCmd(x, first.val, es, ids, kv); ((CallCmd) c).IsFree = isFree; ((CallCmd) c).IsAsync = isAsync; 
-		} else SynErr(125);
+		} else SynErr(126);
 	}
 
 	void Expressions(out List<Expr>/*!*/ es) {
@@ -1480,7 +1480,7 @@ out List<Variable>/*!*/ ins, out List<Variable>/*!*/ outs, out QKeyValue kv) {
 			Get();
 		} else if (la.kind == 59) {
 			Get();
-		} else SynErr(126);
+		} else SynErr(127);
 	}
 
 	void LogicalExpression(out Expr/*!*/ e0) {
@@ -1518,7 +1518,7 @@ out List<Variable>/*!*/ ins, out List<Variable>/*!*/ outs, out QKeyValue kv) {
 			Get();
 		} else if (la.kind == 61) {
 			Get();
-		} else SynErr(127);
+		} else SynErr(128);
 	}
 
 	void ExpliesOp() {
@@ -1526,7 +1526,7 @@ out List<Variable>/*!*/ ins, out List<Variable>/*!*/ outs, out QKeyValue kv) {
 			Get();
 		} else if (la.kind == 63) {
 			Get();
-		} else SynErr(128);
+		} else SynErr(129);
 	}
 
 	void RelationalExpression(out Expr/*!*/ e0) {
@@ -1544,7 +1544,7 @@ out List<Variable>/*!*/ ins, out List<Variable>/*!*/ outs, out QKeyValue kv) {
 			Get();
 		} else if (la.kind == 65) {
 			Get();
-		} else SynErr(129);
+		} else SynErr(130);
 	}
 
 	void OrOp() {
@@ -1552,7 +1552,7 @@ out List<Variable>/*!*/ ins, out List<Variable>/*!*/ outs, out QKeyValue kv) {
 			Get();
 		} else if (la.kind == 67) {
 			Get();
-		} else SynErr(130);
+		} else SynErr(131);
 	}
 
 	void BvTerm(out Expr/*!*/ e0) {
@@ -1619,7 +1619,7 @@ out List<Variable>/*!*/ ins, out List<Variable>/*!*/ outs, out QKeyValue kv) {
 			x = t; op=BinaryOperator.Opcode.Ge; 
 			break;
 		}
-		default: SynErr(131); break;
+		default: SynErr(132); break;
 		}
 	}
 
@@ -1651,7 +1651,7 @@ out List<Variable>/*!*/ ins, out List<Variable>/*!*/ outs, out QKeyValue kv) {
 		} else if (la.kind == 78) {
 			Get();
 			x = t; op=BinaryOperator.Opcode.Sub; 
-		} else SynErr(132);
+		} else SynErr(133);
 	}
 
 	void Power(out Expr/*!*/ e0) {
@@ -1679,11 +1679,11 @@ out List<Variable>/*!*/ ins, out List<Variable>/*!*/ outs, out QKeyValue kv) {
 		} else if (la.kind == 81) {
 			Get();
 			x = t; op=BinaryOperator.Opcode.RealDiv; 
-		} else SynErr(133);
+		} else SynErr(134);
 	}
 
 	void UnaryExpression(out Expr/*!*/ e) {
-		Contract.Ensures(Contract.ValueAtReturn(out e) != null); IToken/*!*/ x;
+		Contract.Ensures(Contract.ValueAtReturn(out e) != null); IToken/*!*/ x; IsConstructor isConstructor;
 		e = dummyExpr;
 		
 		if (la.kind == 78) {
@@ -1698,7 +1698,11 @@ out List<Variable>/*!*/ ins, out List<Variable>/*!*/ outs, out QKeyValue kv) {
 			e = Expr.Unary(x, UnaryOperator.Opcode.Not, e); 
 		} else if (StartOf(15)) {
 			CoercionExpression(out e);
-		} else SynErr(134);
+			if (la.val == "is") {
+				IsConstructor(out x, out isConstructor);
+				e = new NAryExpr(x, isConstructor, new List<Expr> { e }); 
+			}
+		} else SynErr(135);
 	}
 
 	void NegOp() {
@@ -1706,7 +1710,7 @@ out List<Variable>/*!*/ ins, out List<Variable>/*!*/ outs, out QKeyValue kv) {
 			Get();
 		} else if (la.kind == 84) {
 			Get();
-		} else SynErr(135);
+		} else SynErr(136);
 	}
 
 	void CoercionExpression(out Expr/*!*/ e) {
@@ -1730,8 +1734,16 @@ out List<Variable>/*!*/ ins, out List<Variable>/*!*/ outs, out QKeyValue kv) {
 				 e = new BvBounds(x, bn, ((LiteralExpr)e).asBigNum);
 				}
 				
-			} else SynErr(136);
+			} else SynErr(137);
 		}
+	}
+
+	void IsConstructor(out IToken x, out IsConstructor isConstructor) {
+		Contract.Ensures(Contract.ValueAtReturn(out isConstructor) != null); IToken id; 
+		Expect(85);
+		x = t; 
+		Ident(out id);
+		isConstructor = new IsConstructor(id, id.val); 
 	}
 
 	void ArrayExpression(out Expr/*!*/ e) {
@@ -1818,18 +1830,18 @@ out List<Variable>/*!*/ ins, out List<Variable>/*!*/ outs, out QKeyValue kv) {
 		List<Block/*!*/>/*!*/ blocks;
 		
 		switch (la.kind) {
-		case 85: {
+		case 86: {
 			Get();
 			e = new LiteralExpr(t, false); 
 			break;
 		}
-		case 86: {
+		case 87: {
 			Get();
 			e = new LiteralExpr(t, true); 
 			break;
 		}
-		case 87: case 88: {
-			if (la.kind == 87) {
+		case 88: case 89: {
+			if (la.kind == 88) {
 				Get();
 			} else {
 				Get();
@@ -1837,8 +1849,8 @@ out List<Variable>/*!*/ ins, out List<Variable>/*!*/ outs, out QKeyValue kv) {
 			e = new LiteralExpr(t, RoundingMode.RNE); 
 			break;
 		}
-		case 89: case 90: {
-			if (la.kind == 89) {
+		case 90: case 91: {
+			if (la.kind == 90) {
 				Get();
 			} else {
 				Get();
@@ -1846,8 +1858,8 @@ out List<Variable>/*!*/ ins, out List<Variable>/*!*/ outs, out QKeyValue kv) {
 			e = new LiteralExpr(t, RoundingMode.RNA); 
 			break;
 		}
-		case 91: case 92: {
-			if (la.kind == 91) {
+		case 92: case 93: {
+			if (la.kind == 92) {
 				Get();
 			} else {
 				Get();
@@ -1855,8 +1867,8 @@ out List<Variable>/*!*/ ins, out List<Variable>/*!*/ outs, out QKeyValue kv) {
 			e = new LiteralExpr(t, RoundingMode.RTP); 
 			break;
 		}
-		case 93: case 94: {
-			if (la.kind == 93) {
+		case 94: case 95: {
+			if (la.kind == 94) {
 				Get();
 			} else {
 				Get();
@@ -1864,8 +1876,8 @@ out List<Variable>/*!*/ ins, out List<Variable>/*!*/ outs, out QKeyValue kv) {
 			e = new LiteralExpr(t, RoundingMode.RTN); 
 			break;
 		}
-		case 95: case 96: {
-			if (la.kind == 95) {
+		case 96: case 97: {
+			if (la.kind == 96) {
 				Get();
 			} else {
 				Get();
@@ -1908,12 +1920,12 @@ out List<Variable>/*!*/ ins, out List<Variable>/*!*/ outs, out QKeyValue kv) {
 					e = new NAryExpr(x, new FunctionCall(id), es); 
 				} else if (la.kind == 11) {
 					e = new NAryExpr(x, new FunctionCall(id), new List<Expr>()); 
-				} else SynErr(137);
+				} else SynErr(138);
 				Expect(11);
 			}
 			break;
 		}
-		case 97: {
+		case 98: {
 			Get();
 			x = t; 
 			Expect(10);
@@ -1946,19 +1958,19 @@ out List<Variable>/*!*/ ins, out List<Variable>/*!*/ outs, out QKeyValue kv) {
 				Expression(out e);
 				if (e is BvBounds)
 				 this.SemErr("parentheses around bitvector bounds are not allowed"); 
-			} else if (la.kind == 101 || la.kind == 102) {
+			} else if (la.kind == 102 || la.kind == 103) {
 				Forall();
 				x = t; 
 				QuantifierBody(x, out typeParams, out ds, out kv, out trig, out e);
 				if (typeParams.Count + ds.Count > 0)
 				 e = new ForallExpr(x, typeParams, ds, kv, trig, e); 
-			} else if (la.kind == 103 || la.kind == 104) {
+			} else if (la.kind == 104 || la.kind == 105) {
 				Exists();
 				x = t; 
 				QuantifierBody(x, out typeParams, out ds, out kv, out trig, out e);
 				if (typeParams.Count + ds.Count > 0)
 				 e = new ExistsExpr(x, typeParams, ds, kv, trig, e); 
-			} else if (la.kind == 105 || la.kind == 106) {
+			} else if (la.kind == 106 || la.kind == 107) {
 				Lambda();
 				x = t; 
 				QuantifierBody(x, out typeParams, out ds, out kv, out trig, out e);
@@ -1968,7 +1980,7 @@ out List<Variable>/*!*/ ins, out List<Variable>/*!*/ outs, out QKeyValue kv) {
 				 e = new LambdaExpr(x, typeParams, ds, kv, e); 
 			} else if (la.kind == 8) {
 				LetExpr(out e);
-			} else SynErr(138);
+			} else SynErr(139);
 			Expect(11);
 			break;
 		}
@@ -1976,12 +1988,12 @@ out List<Variable>/*!*/ ins, out List<Variable>/*!*/ outs, out QKeyValue kv) {
 			IfThenElseExpression(out e);
 			break;
 		}
-		case 98: {
+		case 99: {
 			CodeExpression(out locals, out blocks);
 			e = new CodeExpr(locals, blocks); 
 			break;
 		}
-		default: SynErr(139); break;
+		default: SynErr(140); break;
 		}
 	}
 
@@ -1993,7 +2005,7 @@ out List<Variable>/*!*/ ins, out List<Variable>/*!*/ outs, out QKeyValue kv) {
 		} else if (la.kind == 6) {
 			Get();
 			s = t.val; 
-		} else SynErr(140);
+		} else SynErr(141);
 		try {
 		 n = BigDec.FromString(s);
 		} catch (FormatException) {
@@ -2033,11 +2045,11 @@ out List<Variable>/*!*/ ins, out List<Variable>/*!*/ outs, out QKeyValue kv) {
 	}
 
 	void Forall() {
-		if (la.kind == 101) {
+		if (la.kind == 102) {
 			Get();
-		} else if (la.kind == 102) {
+		} else if (la.kind == 103) {
 			Get();
-		} else SynErr(141);
+		} else SynErr(142);
 	}
 
 	void QuantifierBody(IToken/*!*/ q, out List<TypeVariable>/*!*/ typeParams, out List<Variable>/*!*/ ds,
@@ -2055,7 +2067,7 @@ out QKeyValue kv, out Trigger trig, out Expr/*!*/ body) {
 			}
 		} else if (la.kind == 1 || la.kind == 25) {
 			BoundVars(out ds);
-		} else SynErr(142);
+		} else SynErr(143);
 		QSep();
 		while (la.kind == 25) {
 			AttributeOrTrigger(ref kv, ref trig);
@@ -2064,19 +2076,19 @@ out QKeyValue kv, out Trigger trig, out Expr/*!*/ body) {
 	}
 
 	void Exists() {
-		if (la.kind == 103) {
+		if (la.kind == 104) {
 			Get();
-		} else if (la.kind == 104) {
+		} else if (la.kind == 105) {
 			Get();
-		} else SynErr(143);
+		} else SynErr(144);
 	}
 
 	void Lambda() {
-		if (la.kind == 105) {
+		if (la.kind == 106) {
 			Get();
-		} else if (la.kind == 106) {
+		} else if (la.kind == 107) {
 			Get();
-		} else SynErr(144);
+		} else SynErr(145);
 	}
 
 	void LetExpr(out Expr/*!*/ letexpr) {
@@ -2121,7 +2133,7 @@ out QKeyValue kv, out Trigger trig, out Expr/*!*/ body) {
 		Expect(42);
 		tok = t; 
 		Expression(out e0);
-		Expect(100);
+		Expect(101);
 		Expression(out e1);
 		Expect(43);
 		Expression(out e2);
@@ -2132,7 +2144,7 @@ out QKeyValue kv, out Trigger trig, out Expr/*!*/ body) {
 		Contract.Ensures(Contract.ValueAtReturn(out locals) != null); Contract.Ensures(cce.NonNullElements(Contract.ValueAtReturn(out blocks))); locals = new List<Variable>(); Block/*!*/ b;
 		blocks = new List<Block/*!*/>();
 		
-		Expect(98);
+		Expect(99);
 		while (la.kind == 8) {
 			LocalVars(locals);
 		}
@@ -2142,7 +2154,7 @@ out QKeyValue kv, out Trigger trig, out Expr/*!*/ body) {
 			SpecBlock(out b);
 			blocks.Add(b); 
 		}
-		Expect(99);
+		Expect(100);
 	}
 
 	void SpecBlock(out Block/*!*/ b) {
@@ -2179,7 +2191,7 @@ out QKeyValue kv, out Trigger trig, out Expr/*!*/ body) {
 			Get();
 			Expression(out e);
 			b = new Block(x,x.val,cs,new ReturnExprCmd(t,e)); 
-		} else SynErr(145);
+		} else SynErr(146);
 		Expect(9);
 	}
 
@@ -2236,7 +2248,7 @@ out QKeyValue kv, out Trigger trig, out Expr/*!*/ body) {
 			 trig.AddLast(new Trigger(tok, true, es, null));
 			}
 			
-		} else SynErr(146);
+		} else SynErr(147);
 		Expect(26);
 	}
 
@@ -2251,15 +2263,15 @@ out QKeyValue kv, out Trigger trig, out Expr/*!*/ body) {
 		} else if (StartOf(9)) {
 			Expression(out e);
 			o = e; 
-		} else SynErr(147);
+		} else SynErr(148);
 	}
 
 	void QSep() {
-		if (la.kind == 107) {
+		if (la.kind == 108) {
 			Get();
-		} else if (la.kind == 108) {
+		} else if (la.kind == 109) {
 			Get();
-		} else SynErr(148);
+		} else SynErr(149);
 	}
 
 	void LetVar(out Variable/*!*/ v) {
@@ -2288,23 +2300,23 @@ out QKeyValue kv, out Trigger trig, out Expr/*!*/ body) {
 	}
 
 	static readonly bool[,]/*!*/ set = {
-		{_T,_x,_x,_x, _x,_x,_x,_x, _x,_x,_x,_x, _x,_x,_x,_x, _x,_x,_x,_x, _x,_x,_x,_x, _x,_x,_x,_x, _x,_x,_x,_x, _x,_x,_x,_x, _x,_x,_x,_x, _x,_x,_x,_x, _x,_x,_x,_x, _x,_x,_x,_x, _x,_x,_x,_x, _x,_x,_x,_x, _x,_x,_x,_x, _x,_x,_x,_x, _x,_x,_x,_x, _x,_x,_x,_x, _x,_x,_x,_x, _x,_x,_x,_x, _x,_x,_x,_x, _x,_x,_x,_x, _x,_x,_x,_x, _x,_x,_x,_x, _x,_x,_x,_x, _x,_x,_x,_x, _x,_x,_x},
-		{_x,_x,_x,_x, _x,_x,_x,_x, _T,_x,_x,_x, _x,_x,_x,_x, _x,_x,_x,_x, _x,_x,_T,_x, _x,_x,_x,_x, _x,_T,_x,_T, _T,_x,_T,_T, _x,_x,_x,_x, _x,_x,_x,_x, _x,_x,_x,_x, _x,_x,_x,_x, _x,_x,_x,_x, _x,_x,_x,_x, _x,_x,_x,_x, _x,_x,_x,_x, _x,_x,_x,_x, _x,_x,_x,_x, _x,_x,_x,_x, _x,_x,_x,_x, _x,_x,_x,_x, _x,_x,_x,_x, _x,_x,_x,_x, _x,_x,_x,_x, _x,_x,_x,_x, _x,_x,_x,_x, _x,_x,_x},
-		{_x,_T,_x,_x, _x,_x,_x,_x, _x,_x,_T,_x, _x,_x,_x,_T, _T,_T,_T,_x, _T,_x,_x,_x, _x,_T,_x,_x, _x,_x,_x,_x, _x,_x,_x,_x, _x,_x,_x,_x, _x,_x,_x,_x, _x,_x,_x,_x, _x,_x,_x,_x, _x,_x,_x,_x, _x,_x,_x,_x, _x,_x,_x,_x, _x,_x,_x,_x, _x,_x,_x,_x, _x,_x,_x,_x, _x,_x,_x,_x, _x,_x,_x,_x, _x,_x,_x,_x, _x,_x,_x,_x, _x,_x,_x,_x, _x,_x,_x,_x, _x,_x,_x,_x, _x,_x,_x,_x, _x,_x,_x},
-		{_x,_x,_x,_x, _x,_x,_x,_x, _x,_x,_x,_x, _x,_x,_x,_x, _x,_x,_x,_x, _x,_x,_x,_x, _x,_x,_x,_x, _x,_x,_x,_x, _x,_x,_x,_x, _T,_T,_T,_T, _x,_x,_x,_x, _x,_x,_x,_x, _x,_x,_x,_x, _x,_x,_x,_x, _x,_x,_x,_x, _x,_x,_x,_x, _x,_x,_x,_x, _x,_x,_x,_x, _x,_x,_x,_x, _x,_x,_x,_x, _x,_x,_x,_x, _x,_x,_x,_x, _x,_x,_x,_x, _x,_x,_x,_x, _x,_x,_x,_x, _x,_x,_x,_x, _x,_x,_x,_x, _x,_x,_x},
-		{_x,_x,_x,_x, _x,_x,_x,_x, _x,_x,_x,_x, _x,_x,_x,_x, _x,_x,_x,_x, _x,_x,_x,_x, _x,_T,_x,_x, _x,_x,_x,_x, _x,_x,_x,_x, _T,_T,_T,_T, _x,_x,_x,_x, _x,_x,_x,_x, _x,_x,_x,_x, _x,_x,_x,_x, _x,_x,_x,_x, _x,_x,_x,_x, _x,_x,_x,_x, _x,_x,_x,_x, _x,_x,_x,_x, _x,_x,_x,_x, _x,_x,_x,_x, _x,_x,_x,_x, _x,_x,_x,_x, _x,_x,_x,_x, _x,_x,_x,_x, _x,_x,_x,_x, _x,_x,_x,_x, _x,_x,_x},
-		{_x,_x,_x,_x, _x,_x,_x,_x, _x,_x,_T,_x, _x,_x,_x,_T, _T,_T,_x,_x, _x,_x,_x,_x, _x,_x,_x,_x, _x,_x,_x,_x, _x,_x,_x,_x, _x,_x,_x,_x, _x,_x,_x,_x, _x,_x,_x,_x, _x,_x,_x,_x, _x,_x,_x,_x, _x,_x,_x,_x, _x,_x,_x,_x, _x,_x,_x,_x, _x,_x,_x,_x, _x,_x,_x,_x, _x,_x,_x,_x, _x,_x,_x,_x, _x,_x,_x,_x, _x,_x,_x,_x, _x,_x,_x,_x, _x,_x,_x,_x, _x,_x,_x,_x, _x,_x,_x,_x, _x,_x,_x},
-		{_x,_T,_x,_x, _x,_x,_x,_x, _x,_x,_T,_x, _x,_x,_x,_T, _T,_T,_T,_x, _T,_x,_x,_x, _x,_x,_x,_x, _x,_x,_x,_x, _x,_x,_x,_x, _x,_x,_x,_x, _x,_x,_x,_x, _x,_x,_x,_x, _x,_x,_x,_x, _x,_x,_x,_x, _x,_x,_x,_x, _x,_x,_x,_x, _x,_x,_x,_x, _x,_x,_x,_x, _x,_x,_x,_x, _x,_x,_x,_x, _x,_x,_x,_x, _x,_x,_x,_x, _x,_x,_x,_x, _x,_x,_x,_x, _x,_x,_x,_x, _x,_x,_x,_x, _x,_x,_x,_x, _x,_x,_x},
-		{_x,_T,_x,_x, _x,_x,_x,_x, _x,_x,_x,_x, _x,_x,_x,_x, _x,_x,_x,_x, _x,_x,_x,_x, _x,_x,_x,_x, _x,_x,_x,_x, _x,_x,_x,_x, _x,_T,_x,_x, _T,_T,_T,_x, _T,_x,_x,_T, _T,_T,_T,_T, _x,_x,_T,_T, _T,_x,_x,_x, _x,_x,_x,_x, _x,_x,_x,_x, _x,_x,_x,_x, _x,_x,_x,_x, _x,_x,_x,_x, _x,_x,_x,_x, _x,_x,_x,_x, _x,_x,_x,_x, _x,_x,_x,_x, _x,_x,_x,_x, _x,_x,_x,_x, _x,_x,_x,_x, _x,_x,_x},
-		{_x,_T,_x,_x, _x,_x,_x,_x, _x,_x,_x,_x, _x,_x,_x,_x, _x,_x,_x,_x, _x,_x,_x,_x, _x,_x,_x,_x, _x,_x,_x,_x, _x,_x,_x,_x, _x,_T,_x,_x, _x,_x,_x,_x, _x,_x,_x,_x, _T,_T,_T,_T, _x,_x,_T,_T, _T,_x,_x,_x, _x,_x,_x,_x, _x,_x,_x,_x, _x,_x,_x,_x, _x,_x,_x,_x, _x,_x,_x,_x, _x,_x,_x,_x, _x,_x,_x,_x, _x,_x,_x,_x, _x,_x,_x,_x, _x,_x,_x,_x, _x,_x,_x,_x, _x,_x,_x,_x, _x,_x,_x},
-		{_x,_T,_T,_T, _T,_T,_T,_T, _x,_x,_T,_x, _x,_x,_x,_T, _T,_x,_x,_x, _x,_x,_x,_x, _x,_x,_x,_x, _x,_x,_x,_x, _x,_x,_x,_x, _x,_x,_x,_x, _x,_x,_T,_x, _x,_x,_x,_x, _x,_x,_x,_x, _x,_x,_x,_x, _x,_x,_x,_x, _x,_x,_x,_x, _x,_x,_x,_x, _x,_x,_x,_x, _x,_x,_x,_x, _x,_x,_T,_x, _x,_x,_x,_T, _T,_T,_T,_T, _T,_T,_T,_T, _T,_T,_T,_T, _T,_T,_T,_x, _x,_x,_x,_x, _x,_x,_x,_x, _x,_x,_x},
-		{_x,_x,_x,_x, _x,_x,_x,_x, _x,_x,_x,_x, _x,_T,_x,_x, _x,_x,_T,_x, _x,_x,_x,_x, _x,_x,_x,_x, _x,_x,_x,_x, _x,_x,_x,_x, _x,_x,_x,_x, _x,_x,_x,_x, _x,_x,_x,_x, _x,_x,_x,_x, _T,_T,_x,_x, _x,_x,_x,_x, _x,_x,_x,_x, _x,_x,_x,_x, _x,_x,_x,_x, _x,_x,_x,_x, _x,_x,_x,_x, _x,_x,_x,_x, _x,_x,_x,_x, _x,_x,_x,_x, _x,_x,_x,_x, _x,_x,_x,_x, _x,_x,_x,_x, _x,_x,_x,_x, _x,_x,_x},
-		{_x,_x,_x,_x, _x,_x,_x,_x, _x,_x,_x,_x, _x,_x,_x,_x, _x,_x,_x,_x, _x,_x,_x,_x, _x,_x,_x,_x, _x,_x,_x,_x, _x,_x,_x,_x, _x,_x,_x,_x, _x,_x,_x,_x, _x,_x,_x,_x, _x,_x,_x,_x, _x,_x,_x,_x, _x,_x,_x,_x, _T,_T,_T,_T, _x,_x,_x,_x, _x,_x,_x,_x, _x,_x,_x,_x, _x,_x,_x,_x, _x,_x,_x,_x, _x,_x,_x,_x, _x,_x,_x,_x, _x,_x,_x,_x, _x,_x,_x,_x, _x,_x,_x,_x, _x,_x,_x,_x, _x,_x,_x},
-		{_x,_x,_x,_x, _x,_x,_x,_x, _x,_x,_x,_x, _x,_x,_x,_x, _x,_x,_x,_x, _x,_x,_x,_x, _x,_x,_x,_x, _x,_x,_x,_x, _x,_x,_x,_x, _x,_x,_x,_x, _x,_x,_x,_x, _x,_x,_x,_x, _x,_x,_x,_x, _x,_x,_x,_x, _x,_x,_x,_x, _x,_x,_x,_x, _T,_T,_T,_T, _x,_x,_x,_x, _x,_x,_x,_x, _x,_x,_x,_x, _x,_x,_x,_x, _x,_x,_x,_x, _x,_x,_x,_x, _x,_x,_x,_x, _x,_x,_x,_x, _x,_x,_x,_x, _x,_x,_x,_x, _x,_x,_x},
-		{_x,_x,_x,_x, _x,_x,_x,_x, _x,_x,_x,_x, _x,_x,_x,_x, _x,_x,_x,_x, _T,_T,_x,_x, _x,_x,_x,_x, _x,_x,_x,_x, _x,_x,_x,_x, _x,_x,_x,_x, _x,_x,_x,_x, _x,_x,_x,_x, _x,_x,_x,_x, _x,_x,_x,_x, _x,_x,_x,_x, _x,_x,_x,_x, _x,_x,_x,_x, _T,_T,_T,_T, _T,_T,_T,_T, _x,_x,_x,_x, _x,_x,_x,_x, _x,_x,_x,_x, _x,_x,_x,_x, _x,_x,_x,_x, _x,_x,_x,_x, _x,_x,_x,_x, _x,_x,_x,_x, _x,_x,_x},
-		{_x,_x,_x,_x, _x,_x,_x,_x, _x,_x,_x,_x, _x,_x,_x,_x, _x,_x,_x,_x, _x,_x,_x,_x, _x,_x,_x,_x, _x,_x,_x,_x, _x,_x,_x,_x, _x,_x,_x,_x, _x,_x,_x,_x, _x,_x,_T,_x, _x,_x,_x,_x, _x,_x,_x,_x, _x,_x,_x,_x, _x,_x,_x,_x, _x,_x,_x,_x, _x,_x,_x,_x, _x,_x,_x,_x, _x,_x,_x,_T, _T,_T,_x,_x, _x,_x,_x,_x, _x,_x,_x,_x, _x,_x,_x,_x, _x,_x,_x,_x, _x,_x,_x,_x, _x,_x,_x,_x, _x,_x,_x},
-		{_x,_T,_T,_T, _T,_T,_T,_T, _x,_x,_T,_x, _x,_x,_x,_T, _T,_x,_x,_x, _x,_x,_x,_x, _x,_x,_x,_x, _x,_x,_x,_x, _x,_x,_x,_x, _x,_x,_x,_x, _x,_x,_T,_x, _x,_x,_x,_x, _x,_x,_x,_x, _x,_x,_x,_x, _x,_x,_x,_x, _x,_x,_x,_x, _x,_x,_x,_x, _x,_x,_x,_x, _x,_x,_x,_x, _x,_x,_x,_x, _x,_x,_x,_x, _x,_T,_T,_T, _T,_T,_T,_T, _T,_T,_T,_T, _T,_T,_T,_x, _x,_x,_x,_x, _x,_x,_x,_x, _x,_x,_x},
-		{_x,_T,_T,_T, _T,_T,_T,_T, _x,_x,_T,_x, _x,_x,_x,_T, _T,_x,_x,_x, _x,_x,_x,_x, _x,_x,_x,_x, _x,_x,_x,_x, _x,_x,_x,_x, _x,_x,_x,_x, _x,_x,_T,_x, _x,_x,_x,_x, _x,_x,_x,_x, _T,_x,_x,_x, _x,_x,_x,_x, _x,_x,_x,_x, _x,_x,_x,_x, _x,_x,_x,_x, _x,_x,_x,_x, _x,_x,_T,_x, _x,_x,_x,_T, _T,_T,_T,_T, _T,_T,_T,_T, _T,_T,_T,_T, _T,_T,_T,_x, _x,_x,_x,_x, _x,_x,_x,_x, _x,_x,_x}
+		{_T,_x,_x,_x, _x,_x,_x,_x, _x,_x,_x,_x, _x,_x,_x,_x, _x,_x,_x,_x, _x,_x,_x,_x, _x,_x,_x,_x, _x,_x,_x,_x, _x,_x,_x,_x, _x,_x,_x,_x, _x,_x,_x,_x, _x,_x,_x,_x, _x,_x,_x,_x, _x,_x,_x,_x, _x,_x,_x,_x, _x,_x,_x,_x, _x,_x,_x,_x, _x,_x,_x,_x, _x,_x,_x,_x, _x,_x,_x,_x, _x,_x,_x,_x, _x,_x,_x,_x, _x,_x,_x,_x, _x,_x,_x,_x, _x,_x,_x,_x, _x,_x,_x,_x, _x,_x,_x,_x, _x,_x,_x,_x},
+		{_x,_x,_x,_x, _x,_x,_x,_x, _T,_x,_x,_x, _x,_x,_x,_x, _x,_x,_x,_x, _x,_x,_T,_x, _x,_x,_x,_x, _x,_T,_x,_T, _T,_x,_T,_T, _x,_x,_x,_x, _x,_x,_x,_x, _x,_x,_x,_x, _x,_x,_x,_x, _x,_x,_x,_x, _x,_x,_x,_x, _x,_x,_x,_x, _x,_x,_x,_x, _x,_x,_x,_x, _x,_x,_x,_x, _x,_x,_x,_x, _x,_x,_x,_x, _x,_x,_x,_x, _x,_x,_x,_x, _x,_x,_x,_x, _x,_x,_x,_x, _x,_x,_x,_x, _x,_x,_x,_x, _x,_x,_x,_x},
+		{_x,_T,_x,_x, _x,_x,_x,_x, _x,_x,_T,_x, _x,_x,_x,_T, _T,_T,_T,_x, _T,_x,_x,_x, _x,_T,_x,_x, _x,_x,_x,_x, _x,_x,_x,_x, _x,_x,_x,_x, _x,_x,_x,_x, _x,_x,_x,_x, _x,_x,_x,_x, _x,_x,_x,_x, _x,_x,_x,_x, _x,_x,_x,_x, _x,_x,_x,_x, _x,_x,_x,_x, _x,_x,_x,_x, _x,_x,_x,_x, _x,_x,_x,_x, _x,_x,_x,_x, _x,_x,_x,_x, _x,_x,_x,_x, _x,_x,_x,_x, _x,_x,_x,_x, _x,_x,_x,_x, _x,_x,_x,_x},
+		{_x,_x,_x,_x, _x,_x,_x,_x, _x,_x,_x,_x, _x,_x,_x,_x, _x,_x,_x,_x, _x,_x,_x,_x, _x,_x,_x,_x, _x,_x,_x,_x, _x,_x,_x,_x, _T,_T,_T,_T, _x,_x,_x,_x, _x,_x,_x,_x, _x,_x,_x,_x, _x,_x,_x,_x, _x,_x,_x,_x, _x,_x,_x,_x, _x,_x,_x,_x, _x,_x,_x,_x, _x,_x,_x,_x, _x,_x,_x,_x, _x,_x,_x,_x, _x,_x,_x,_x, _x,_x,_x,_x, _x,_x,_x,_x, _x,_x,_x,_x, _x,_x,_x,_x, _x,_x,_x,_x, _x,_x,_x,_x},
+		{_x,_x,_x,_x, _x,_x,_x,_x, _x,_x,_x,_x, _x,_x,_x,_x, _x,_x,_x,_x, _x,_x,_x,_x, _x,_T,_x,_x, _x,_x,_x,_x, _x,_x,_x,_x, _T,_T,_T,_T, _x,_x,_x,_x, _x,_x,_x,_x, _x,_x,_x,_x, _x,_x,_x,_x, _x,_x,_x,_x, _x,_x,_x,_x, _x,_x,_x,_x, _x,_x,_x,_x, _x,_x,_x,_x, _x,_x,_x,_x, _x,_x,_x,_x, _x,_x,_x,_x, _x,_x,_x,_x, _x,_x,_x,_x, _x,_x,_x,_x, _x,_x,_x,_x, _x,_x,_x,_x, _x,_x,_x,_x},
+		{_x,_x,_x,_x, _x,_x,_x,_x, _x,_x,_T,_x, _x,_x,_x,_T, _T,_T,_x,_x, _x,_x,_x,_x, _x,_x,_x,_x, _x,_x,_x,_x, _x,_x,_x,_x, _x,_x,_x,_x, _x,_x,_x,_x, _x,_x,_x,_x, _x,_x,_x,_x, _x,_x,_x,_x, _x,_x,_x,_x, _x,_x,_x,_x, _x,_x,_x,_x, _x,_x,_x,_x, _x,_x,_x,_x, _x,_x,_x,_x, _x,_x,_x,_x, _x,_x,_x,_x, _x,_x,_x,_x, _x,_x,_x,_x, _x,_x,_x,_x, _x,_x,_x,_x, _x,_x,_x,_x, _x,_x,_x,_x},
+		{_x,_T,_x,_x, _x,_x,_x,_x, _x,_x,_T,_x, _x,_x,_x,_T, _T,_T,_T,_x, _T,_x,_x,_x, _x,_x,_x,_x, _x,_x,_x,_x, _x,_x,_x,_x, _x,_x,_x,_x, _x,_x,_x,_x, _x,_x,_x,_x, _x,_x,_x,_x, _x,_x,_x,_x, _x,_x,_x,_x, _x,_x,_x,_x, _x,_x,_x,_x, _x,_x,_x,_x, _x,_x,_x,_x, _x,_x,_x,_x, _x,_x,_x,_x, _x,_x,_x,_x, _x,_x,_x,_x, _x,_x,_x,_x, _x,_x,_x,_x, _x,_x,_x,_x, _x,_x,_x,_x, _x,_x,_x,_x},
+		{_x,_T,_x,_x, _x,_x,_x,_x, _x,_x,_x,_x, _x,_x,_x,_x, _x,_x,_x,_x, _x,_x,_x,_x, _x,_x,_x,_x, _x,_x,_x,_x, _x,_x,_x,_x, _x,_T,_x,_x, _T,_T,_T,_x, _T,_x,_x,_T, _T,_T,_T,_T, _x,_x,_T,_T, _T,_x,_x,_x, _x,_x,_x,_x, _x,_x,_x,_x, _x,_x,_x,_x, _x,_x,_x,_x, _x,_x,_x,_x, _x,_x,_x,_x, _x,_x,_x,_x, _x,_x,_x,_x, _x,_x,_x,_x, _x,_x,_x,_x, _x,_x,_x,_x, _x,_x,_x,_x, _x,_x,_x,_x},
+		{_x,_T,_x,_x, _x,_x,_x,_x, _x,_x,_x,_x, _x,_x,_x,_x, _x,_x,_x,_x, _x,_x,_x,_x, _x,_x,_x,_x, _x,_x,_x,_x, _x,_x,_x,_x, _x,_T,_x,_x, _x,_x,_x,_x, _x,_x,_x,_x, _T,_T,_T,_T, _x,_x,_T,_T, _T,_x,_x,_x, _x,_x,_x,_x, _x,_x,_x,_x, _x,_x,_x,_x, _x,_x,_x,_x, _x,_x,_x,_x, _x,_x,_x,_x, _x,_x,_x,_x, _x,_x,_x,_x, _x,_x,_x,_x, _x,_x,_x,_x, _x,_x,_x,_x, _x,_x,_x,_x, _x,_x,_x,_x},
+		{_x,_T,_T,_T, _T,_T,_T,_T, _x,_x,_T,_x, _x,_x,_x,_T, _T,_x,_x,_x, _x,_x,_x,_x, _x,_x,_x,_x, _x,_x,_x,_x, _x,_x,_x,_x, _x,_x,_x,_x, _x,_x,_T,_x, _x,_x,_x,_x, _x,_x,_x,_x, _x,_x,_x,_x, _x,_x,_x,_x, _x,_x,_x,_x, _x,_x,_x,_x, _x,_x,_x,_x, _x,_x,_x,_x, _x,_x,_T,_x, _x,_x,_x,_T, _T,_x,_T,_T, _T,_T,_T,_T, _T,_T,_T,_T, _T,_T,_T,_T, _x,_x,_x,_x, _x,_x,_x,_x, _x,_x,_x,_x},
+		{_x,_x,_x,_x, _x,_x,_x,_x, _x,_x,_x,_x, _x,_T,_x,_x, _x,_x,_T,_x, _x,_x,_x,_x, _x,_x,_x,_x, _x,_x,_x,_x, _x,_x,_x,_x, _x,_x,_x,_x, _x,_x,_x,_x, _x,_x,_x,_x, _x,_x,_x,_x, _T,_T,_x,_x, _x,_x,_x,_x, _x,_x,_x,_x, _x,_x,_x,_x, _x,_x,_x,_x, _x,_x,_x,_x, _x,_x,_x,_x, _x,_x,_x,_x, _x,_x,_x,_x, _x,_x,_x,_x, _x,_x,_x,_x, _x,_x,_x,_x, _x,_x,_x,_x, _x,_x,_x,_x, _x,_x,_x,_x},
+		{_x,_x,_x,_x, _x,_x,_x,_x, _x,_x,_x,_x, _x,_x,_x,_x, _x,_x,_x,_x, _x,_x,_x,_x, _x,_x,_x,_x, _x,_x,_x,_x, _x,_x,_x,_x, _x,_x,_x,_x, _x,_x,_x,_x, _x,_x,_x,_x, _x,_x,_x,_x, _x,_x,_x,_x, _x,_x,_x,_x, _T,_T,_T,_T, _x,_x,_x,_x, _x,_x,_x,_x, _x,_x,_x,_x, _x,_x,_x,_x, _x,_x,_x,_x, _x,_x,_x,_x, _x,_x,_x,_x, _x,_x,_x,_x, _x,_x,_x,_x, _x,_x,_x,_x, _x,_x,_x,_x, _x,_x,_x,_x},
+		{_x,_x,_x,_x, _x,_x,_x,_x, _x,_x,_x,_x, _x,_x,_x,_x, _x,_x,_x,_x, _x,_x,_x,_x, _x,_x,_x,_x, _x,_x,_x,_x, _x,_x,_x,_x, _x,_x,_x,_x, _x,_x,_x,_x, _x,_x,_x,_x, _x,_x,_x,_x, _x,_x,_x,_x, _x,_x,_x,_x, _x,_x,_x,_x, _T,_T,_T,_T, _x,_x,_x,_x, _x,_x,_x,_x, _x,_x,_x,_x, _x,_x,_x,_x, _x,_x,_x,_x, _x,_x,_x,_x, _x,_x,_x,_x, _x,_x,_x,_x, _x,_x,_x,_x, _x,_x,_x,_x, _x,_x,_x,_x},
+		{_x,_x,_x,_x, _x,_x,_x,_x, _x,_x,_x,_x, _x,_x,_x,_x, _x,_x,_x,_x, _T,_T,_x,_x, _x,_x,_x,_x, _x,_x,_x,_x, _x,_x,_x,_x, _x,_x,_x,_x, _x,_x,_x,_x, _x,_x,_x,_x, _x,_x,_x,_x, _x,_x,_x,_x, _x,_x,_x,_x, _x,_x,_x,_x, _x,_x,_x,_x, _T,_T,_T,_T, _T,_T,_T,_T, _x,_x,_x,_x, _x,_x,_x,_x, _x,_x,_x,_x, _x,_x,_x,_x, _x,_x,_x,_x, _x,_x,_x,_x, _x,_x,_x,_x, _x,_x,_x,_x, _x,_x,_x,_x},
+		{_x,_x,_x,_x, _x,_x,_x,_x, _x,_x,_x,_x, _x,_x,_x,_x, _x,_x,_x,_x, _x,_x,_x,_x, _x,_x,_x,_x, _x,_x,_x,_x, _x,_x,_x,_x, _x,_x,_x,_x, _x,_x,_x,_x, _x,_x,_T,_x, _x,_x,_x,_x, _x,_x,_x,_x, _x,_x,_x,_x, _x,_x,_x,_x, _x,_x,_x,_x, _x,_x,_x,_x, _x,_x,_x,_x, _x,_x,_x,_T, _T,_T,_x,_x, _x,_x,_x,_x, _x,_x,_x,_x, _x,_x,_x,_x, _x,_x,_x,_x, _x,_x,_x,_x, _x,_x,_x,_x, _x,_x,_x,_x},
+		{_x,_T,_T,_T, _T,_T,_T,_T, _x,_x,_T,_x, _x,_x,_x,_T, _T,_x,_x,_x, _x,_x,_x,_x, _x,_x,_x,_x, _x,_x,_x,_x, _x,_x,_x,_x, _x,_x,_x,_x, _x,_x,_T,_x, _x,_x,_x,_x, _x,_x,_x,_x, _x,_x,_x,_x, _x,_x,_x,_x, _x,_x,_x,_x, _x,_x,_x,_x, _x,_x,_x,_x, _x,_x,_x,_x, _x,_x,_x,_x, _x,_x,_x,_x, _x,_x,_T,_T, _T,_T,_T,_T, _T,_T,_T,_T, _T,_T,_T,_T, _x,_x,_x,_x, _x,_x,_x,_x, _x,_x,_x,_x},
+		{_x,_T,_T,_T, _T,_T,_T,_T, _x,_x,_T,_x, _x,_x,_x,_T, _T,_x,_x,_x, _x,_x,_x,_x, _x,_x,_x,_x, _x,_x,_x,_x, _x,_x,_x,_x, _x,_x,_x,_x, _x,_x,_T,_x, _x,_x,_x,_x, _x,_x,_x,_x, _T,_x,_x,_x, _x,_x,_x,_x, _x,_x,_x,_x, _x,_x,_x,_x, _x,_x,_x,_x, _x,_x,_x,_x, _x,_x,_T,_x, _x,_x,_x,_T, _T,_x,_T,_T, _T,_T,_T,_T, _T,_T,_T,_T, _T,_T,_T,_T, _x,_x,_x,_x, _x,_x,_x,_x, _x,_x,_x,_x}
 
 	};
 } // end Parser
@@ -2414,70 +2426,71 @@ public class Errors {
 			case 82: s = "\"**\" expected"; break;
 			case 83: s = "\"!\" expected"; break;
 			case 84: s = "\"\\u00ac\" expected"; break;
-			case 85: s = "\"false\" expected"; break;
-			case 86: s = "\"true\" expected"; break;
-			case 87: s = "\"roundNearestTiesToEven\" expected"; break;
-			case 88: s = "\"RNE\" expected"; break;
-			case 89: s = "\"roundNearestTiesToAway\" expected"; break;
-			case 90: s = "\"RNA\" expected"; break;
-			case 91: s = "\"roundTowardPositive\" expected"; break;
-			case 92: s = "\"RTP\" expected"; break;
-			case 93: s = "\"roundTowardNegative\" expected"; break;
-			case 94: s = "\"RTN\" expected"; break;
-			case 95: s = "\"roundTowardZero\" expected"; break;
-			case 96: s = "\"RTZ\" expected"; break;
-			case 97: s = "\"old\" expected"; break;
-			case 98: s = "\"|{\" expected"; break;
-			case 99: s = "\"}|\" expected"; break;
-			case 100: s = "\"then\" expected"; break;
-			case 101: s = "\"forall\" expected"; break;
-			case 102: s = "\"\\u2200\" expected"; break;
-			case 103: s = "\"exists\" expected"; break;
-			case 104: s = "\"\\u2203\" expected"; break;
-			case 105: s = "\"lambda\" expected"; break;
-			case 106: s = "\"\\u03bb\" expected"; break;
-			case 107: s = "\"::\" expected"; break;
-			case 108: s = "\"\\u2022\" expected"; break;
-			case 109: s = "??? expected"; break;
-			case 110: s = "invalid Consts"; break;
-			case 111: s = "invalid Function"; break;
+			case 85: s = "\"is\" expected"; break;
+			case 86: s = "\"false\" expected"; break;
+			case 87: s = "\"true\" expected"; break;
+			case 88: s = "\"roundNearestTiesToEven\" expected"; break;
+			case 89: s = "\"RNE\" expected"; break;
+			case 90: s = "\"roundNearestTiesToAway\" expected"; break;
+			case 91: s = "\"RNA\" expected"; break;
+			case 92: s = "\"roundTowardPositive\" expected"; break;
+			case 93: s = "\"RTP\" expected"; break;
+			case 94: s = "\"roundTowardNegative\" expected"; break;
+			case 95: s = "\"RTN\" expected"; break;
+			case 96: s = "\"roundTowardZero\" expected"; break;
+			case 97: s = "\"RTZ\" expected"; break;
+			case 98: s = "\"old\" expected"; break;
+			case 99: s = "\"|{\" expected"; break;
+			case 100: s = "\"}|\" expected"; break;
+			case 101: s = "\"then\" expected"; break;
+			case 102: s = "\"forall\" expected"; break;
+			case 103: s = "\"\\u2200\" expected"; break;
+			case 104: s = "\"exists\" expected"; break;
+			case 105: s = "\"\\u2203\" expected"; break;
+			case 106: s = "\"lambda\" expected"; break;
+			case 107: s = "\"\\u03bb\" expected"; break;
+			case 108: s = "\"::\" expected"; break;
+			case 109: s = "\"\\u2022\" expected"; break;
+			case 110: s = "??? expected"; break;
+			case 111: s = "invalid Consts"; break;
 			case 112: s = "invalid Function"; break;
-			case 113: s = "invalid Procedure"; break;
-			case 114: s = "invalid Type"; break;
-			case 115: s = "invalid TypeAtom"; break;
-			case 116: s = "invalid TypeArgs"; break;
-			case 117: s = "invalid Spec"; break;
-			case 118: s = "invalid SpecPrePost"; break;
-			case 119: s = "invalid LabelOrCmd"; break;
-			case 120: s = "invalid StructuredCmd"; break;
-			case 121: s = "invalid TransferCmd"; break;
-			case 122: s = "invalid IfCmd"; break;
-			case 123: s = "invalid Guard"; break;
-			case 124: s = "invalid LabelOrAssign"; break;
-			case 125: s = "invalid CallParams"; break;
-			case 126: s = "invalid EquivOp"; break;
-			case 127: s = "invalid ImpliesOp"; break;
-			case 128: s = "invalid ExpliesOp"; break;
-			case 129: s = "invalid AndOp"; break;
-			case 130: s = "invalid OrOp"; break;
-			case 131: s = "invalid RelOp"; break;
-			case 132: s = "invalid AddOp"; break;
-			case 133: s = "invalid MulOp"; break;
-			case 134: s = "invalid UnaryExpression"; break;
-			case 135: s = "invalid NegOp"; break;
-			case 136: s = "invalid CoercionExpression"; break;
-			case 137: s = "invalid AtomExpression"; break;
+			case 113: s = "invalid Function"; break;
+			case 114: s = "invalid Procedure"; break;
+			case 115: s = "invalid Type"; break;
+			case 116: s = "invalid TypeAtom"; break;
+			case 117: s = "invalid TypeArgs"; break;
+			case 118: s = "invalid Spec"; break;
+			case 119: s = "invalid SpecPrePost"; break;
+			case 120: s = "invalid LabelOrCmd"; break;
+			case 121: s = "invalid StructuredCmd"; break;
+			case 122: s = "invalid TransferCmd"; break;
+			case 123: s = "invalid IfCmd"; break;
+			case 124: s = "invalid Guard"; break;
+			case 125: s = "invalid LabelOrAssign"; break;
+			case 126: s = "invalid CallParams"; break;
+			case 127: s = "invalid EquivOp"; break;
+			case 128: s = "invalid ImpliesOp"; break;
+			case 129: s = "invalid ExpliesOp"; break;
+			case 130: s = "invalid AndOp"; break;
+			case 131: s = "invalid OrOp"; break;
+			case 132: s = "invalid RelOp"; break;
+			case 133: s = "invalid AddOp"; break;
+			case 134: s = "invalid MulOp"; break;
+			case 135: s = "invalid UnaryExpression"; break;
+			case 136: s = "invalid NegOp"; break;
+			case 137: s = "invalid CoercionExpression"; break;
 			case 138: s = "invalid AtomExpression"; break;
 			case 139: s = "invalid AtomExpression"; break;
-			case 140: s = "invalid Dec"; break;
-			case 141: s = "invalid Forall"; break;
-			case 142: s = "invalid QuantifierBody"; break;
-			case 143: s = "invalid Exists"; break;
-			case 144: s = "invalid Lambda"; break;
-			case 145: s = "invalid SpecBlock"; break;
-			case 146: s = "invalid AttributeOrTrigger"; break;
-			case 147: s = "invalid AttributeParameter"; break;
-			case 148: s = "invalid QSep"; break;
+			case 140: s = "invalid AtomExpression"; break;
+			case 141: s = "invalid Dec"; break;
+			case 142: s = "invalid Forall"; break;
+			case 143: s = "invalid QuantifierBody"; break;
+			case 144: s = "invalid Exists"; break;
+			case 145: s = "invalid Lambda"; break;
+			case 146: s = "invalid SpecBlock"; break;
+			case 147: s = "invalid AttributeOrTrigger"; break;
+			case 148: s = "invalid AttributeParameter"; break;
+			case 149: s = "invalid QSep"; break;
 
 			default: s = "error " + n; break;
 		}
