Test/datatypes/field_access_type_error.bpl
@@ -1,13 +1,16 @@
 // RUN: %parallel-boogie "%s" > "%t"
 // RUN: %diff "%s.expect" "%t"
 
+type T;
+
 procedure A(a: int);
 requires a->f == 0;
+requires a is T;
 
 
-type T;
 procedure B(a: T);
 requires a->f == 0;
+requires a is T;
 
 
 type {:datatype} Perm;
@@ -16,6 +19,7 @@ function {:constructor} Right(i: int): Perm;
 
 procedure C(a: Perm);
 requires a->f == 0;
+requires a is Middle;
 
 procedure D(a: Perm);
 requires a->i == 0;
