Test/datatypes/field_type_error.bpl
@@ -1,0 +1,6 @@
+// RUN: %parallel-boogie /monomorphize "%s" > "%t"
+// RUN: %diff "%s.expect" "%t"
+
+type{:datatype} Split _ _;
+function{:constructor} Left<T, U>(i: T, j: U): Split T U;
+function{:constructor} Right<X, Y>(i: Y, k: X): Split X Y;
